StackTyping.dfy
@@ -61,3 +61,75 @@ function method TypeCommands(cs: List<command>, S: Sigma): Maybe<Sigma>
     case Cons(c, cs) =>
       BindMaybe(TypeCommand(c, S), S' => TypeCommands(cs, S'))
 }
+
+function method Split<A>(n: nat, v: seq<A>): (seq<A>, seq<A>)
+  requires n <= |v|
+  ensures var (xs, ys) := Split(n, v); |xs| == n && |ys| == |v| - n
+{
+  var xs := v[.. n];
+  var ys := v[n ..];
+  (xs, ys)
+}
+
+function method Uncons<A>(v: seq<A>): (A, seq<A>)
+  requires 0 < |v|
+  ensures |Uncons(v).1| == |v| - 1
+{
+  var (xs, ys) := Split(1, v);
+  (xs[0], ys)
+}
+
+predicate method TypeJump(D: Delta, SigmaH: Sigma, j: jump, P: Phi) {
+  match j
+    case goto(n) =>
+      n in D && P == D[n]
+    case halt =>
+      0 < |P.out| &&
+      var ((PhiR', SigmaH'), Phi_rest) := Uncons(P.out);
+      SigmaH' == SigmaH
+    case branch(n1, n2) =>
+      0 < |P.out| &&
+      n1 in D && n2 in D &&
+      var ((PhiR, S), Phi_rest) := Uncons(P.out);
+      S != [] &&
+      var (t, S') := Uncons(S);
+      t == Bool &&
+      var P' := Phi([(PhiR, S')] + Phi_rest);
+      D[n1] == D[n2] == P'
+    case call(n, nJ, nR) =>
+      0 < |P.out| &&
+      nJ in D && nR in D &&
+      var ((PhiR, S), Phi_rest) := Uncons(P.out);
+      n < |S| &&
+      var (S1, S2) := Split(n, S);
+      D[nJ] == Phi([(D[nR], S1), (PhiR, S2)] + Phi_rest)
+    case ret(n) =>
+      |P.out| >= 2 &&
+      var ((Phi(PhiR_now), SS), Phi_rest) := Uncons(P.out);
+      n <= |SS| &&
+      var (S_check, S_nope) := Split(n, SS);
+      var ((PhiR,  S),   Phi_rest')  := Uncons(Phi_rest);
+      0 < |PhiR_now| &&
+      var ((PhiR', SS'), Phi_rest'') := Uncons(PhiR_now);
+      n <= |SS'| &&
+      var (S_check', S') := Split(n, SS');
+      S == S' &&
+      S_check == S_check' &&
+      PhiR == PhiR' &&
+      Phi_rest' == Phi_rest''
+}
+
+predicate method TypeBlock(D: Delta, SigmaH: Sigma, b: block, P: Phi) {
+  var (cs, j) := b;
+  0 < |P.out| &&
+  var ((PhiR, S), P_rest) := Uncons(P.out);
+  match TypeCommands(cs, S)
+    case Nothing => false
+    case Just(S') => TypeJump(D, SigmaH, j, Phi([(PhiR, S')] + P_rest))
+}
+
+// What I want:
+//    - pattern matching on sequences using literal and slice notation
+//    - non-linear patterns?
+//    - maybe something like "if pat := exp then ... else ..."? or case defaults?
+//    From these, we get the ability to succinctly match against structure that we need.
